# 数字信号处理B

**PB21511897	李霄奕**

## HW3

### Exercise 1

#### (1)

$$
\begin{align*}
Y_1(k)&=\sum_{n=0}^{2N-1}y_1(n)e^{-j\frac{2\pi}{2N}nk}\quad k=0,1,...,2N-1\\
&=\sum_{n为偶数}x(\dfrac{n}{2})e^{-j\frac{2\pi}{2N}nk}\\
&\text{令}n=2i\\
&=\sum_{i=0}^{N-1}x(i)e^{-j\frac{2\pi}{N}ik}\\
&=X_1(k)\quad k=0,1,...,2N-1\\
&=\begin{cases}
X_1(k)\quad k=0,1,...,N-1\\
X_1(k-N)\quad k=N,N+1,..,2N-1
\end{cases}
\end{align*}
$$



#### (2)

$$
y_2(n)=x(N-1-n)\\
\begin{align*}
Y_2(k)&=\sum_{n=0}^{N-1}y_2(n)e^{-j\frac{2\pi}{N}nk}\quad k=0,1,...,N-1\\
&=\sum_{n=0}^{N-1}x(N-1-n)e^{-j\frac{2\pi}{N}nk}\\
&\text{令}i=N-1-n\\
&=\sum_{i=0}^{N-1}x(i)e^{-j\frac{2\pi}{N}(N-1-i)k}\\
&=e^{-j\frac{2\pi}{N}(N-1)k}\sum_{i=0}^{N-1}x(i)e^{-j\frac{2\pi}{N}i(-k)}\\
&=e^{-j\frac{2\pi}{N}(N-1)k}X(-k)\\
&=e^{-j\frac{2\pi}{N}(N-1)k}X^*(k)\\
\end{align*}\\
$$

$$
y_3(n)=(-1)^nx(n)\\
\begin{align*}
Y_3(k)&=\sum_{n=0}^{N-1}y_3(n)e^{-j\frac{2\pi}{N}nk}\quad k=0,1,...,N-1\\
&=\sum_{n=0}^{N-1}(-1)^nx(n)e^{-j\frac{2\pi}{N}nk}\\
&=\sum_{n=0}^{N-1}x(n)e^{-j\frac{2\pi}{N}nk-j\pi n}\\
&=\sum_{n=0}^{N-1}x(n)e^{-j\frac{2\pi}{N}n(k+N/2)}\\
&=X(k+N/2)
\end{align*}\\
$$

### Exercise 2

$$
\begin{align*}
\sum_{n=0}^{N-1}|x(n)|^2&=\sum_{n=0}^{N-1}x(n)x^*(n)\\
&=\sum_{n=0}^{N-1}x(n)\left(\dfrac{1}{N}\sum_{k=0}^{N-1}X^*(k)W_N^{-kn}\right)\\
&=\dfrac{1}{N}\sum_{k=0}^{N-1}X^*(k)\left(\sum_{n=0}^{N-1}x(n)W_N^{-kn}\right)\\
&=\dfrac{1}{N}\sum_{k=0}^{N-1}X(k)X^*(k)\\
&=\dfrac{1}{N}\sum_{k=0}^{N-1}|X(k)|^2\\
\end{align*}
$$

### Exercise 3

$$
\begin{align*}
\sum_{n=0}^{N-1}x(n)y^*(n)&=\sum_{n=0}^{N-1}x(n)y^*(n)\\
&=\sum_{n=0}^{N-1}x(n)\left(\dfrac{1}{N}\sum_{k=0}^{N-1}Y^*(k)W_N^{-kn}\right)\\
&=\dfrac{1}{N}\sum_{k=0}^{N-1}Y^*(k)\left(\sum_{n=0}^{N-1}x(n)W_N^{-kn}\right)\\
&=\dfrac{1}{N}\sum_{k=0}^{N-1}X(k)Y^*(k)\\
\end{align*}
$$

